\footnotesize
\fancyhead[C]{\itГлава 10}
\linespread{1}
\normalsize
Заключение от $n$ к $n+1$: в силу теорем 111, 107 и 172, имеем
\begin{center}
$(fg)^{(n+1)}=((fg)^{(n)})'=$
\end{center}
\begin{left}
\;\;\;\;\;\;\;\;\;\;\;\;\;\;$=\Big(\sum\limits^n_{\nu=0}\Big(\frac{n}{\nu}\Big)f^{(n-\nu)}g^{(\nu)}\Big)'=\sum\limits^n_{\nu=0}\Big(\frac{n}{\nu}\Big)(f^{(n-\nu)}g^{(\nu)})'=$
\end{left}
\newline
\newline
\begin{left}
\;\;\;\;\;\;\;\;\;\;\;\;\;\;$=\sum\limits^n_{\nu=0}\Big(\frac{n}{\nu}\Big)(f^{(n-\nu+1)}g^{(\nu)}+f^{(n-\nu)}g^{(\nu+1)})=$
\end{left}
\newline
\newline
\begin{left}
\;\;\;\;\;\;\;\;\;\;\;\;\;\;$=\sum\limits^n_{\nu=0}\Big(\frac{n}{\nu}\Big)f^{(n-\nu+1)}g^{(\nu)}+\sum\limits^n_{\nu=0}\Big(\frac{n}{\nu}\Big)f^{(n-\nu)}g^{(\nu+1)}=$
\end{left}
\newline
\newline
\begin{left}
\;\;\;\;\;\;\;\;\;\;\;\;\;\;$=\sum\limits^n_{\nu=0}\Big(\frac{n}{\nu}\Big)f^{(n-\nu+1)}g^{(\nu)}+\sum\limits^{n+1}_{\nu=1}\Big(\frac{n}{\nu-1}\Big)f^{(n-\nu+1)}g^{(\nu)}=$
\newline
\newline
$=f^{(n+1)}g^{(0)}+\sum\limits^n_{\nu=1}\Big(\Big(\frac{n}{\nu}\Big)+\Big(\frac{n}{\nu-1}\Big)\Big)f^{(n+1-\nu)}g^{(\nu)}+f^{(0)}g^{(n+1)}$
\end{left}
\newline
\newline
(последняя $\sum$ в случае $n=0$ означает 0)
\newline
\newline
\begin{left}
\;\;\;\;\;\;\;\;\;\;\;\;\;\;$=\sum\limits^{n+1}_{\nu=0}\Big(\frac{n+1}{\nu}\Big)f^{(n+1-\nu)}g^{(\nu)}$.
\end{left}
\newline
\newline
\begin{left}\;\;\;\;\small{\textsf{\textbf{\textsc{Пример.}}}}\end{left}
\begin{center}
$(fg)'''=f'''g+3f''g'+3f'g''+fg''',$
\end{center}
если $f'''\,$ и $\,g'''$ существуют.
\newline
\newline
\begin{left}\;\;\;\;\small{\textsf{\textbf{\textsc{Теорема 174.}}}}\end{left}
\begin{center}
$(f(cx))^{(n)}=c^nf^{(n)}(cx),$
\end{center}
\textit{если правая часть имеет смысл.}
\par\text{Д\thispace\thinspaceо\thispace\thinspaceк\thispace\thinspaceа\thispace\thinspaceз\thispace\thinspaceа\thispace\thinspaceт\thispace\thinspaceе\thispace\thinspaceл\thispace\thinspaceь\thispace\thinspaceс\thispace\thinspaceт\thispace\thinspaceв\thispace\thinspaceо.}
$\;\,\,$Для$\;\,\,$ $n=0$ --- ясно.$\;\,\,$Заключение$\;\,\,$ от $n$ к $n+1$: по теореме 101,
\[
(f^{(n)}(cx))'=cf^{(n+1)}(cx),
\]
следовательно,
\[
c^{n+1}f^{(n+1)}(cx)=c^n(f^{(n)}(cx))'=(c^nf^{(n)}(cx))'=

\;\;\;\;\;\;\;\;\;\;\;\;\;\;\;\;\;\;\;\;\;\;\;\;\;\;\;\;\;\;\;\,=((f(cx))^{(n)})'=(f(cx))^{(n+1)},
\]
\newpage